Imps/Imp/ImpSyntax.v
@@ -1,0 +1,117 @@
+Add LoadPath "~/Code/Coq".
+
+Require Export Recdef.
+
+Require Export FormalSystems.Base.
+
+Inductive AExp : Type :=
+    | AConst : nat -> AExp
+    | Var : Loc -> AExp
+    | ABinOp : (nat -> nat -> nat) -> AExp -> AExp -> AExp.
+
+Inductive BExp : Type :=
+    | BConst : bool -> BExp
+    | BRelOp : (nat -> nat -> bool) -> AExp -> AExp -> BExp
+    | Not : BExp -> BExp
+    | BBinOp : (bool -> bool -> bool) -> BExp -> BExp -> BExp.
+
+Inductive Com : Type :=
+    | Skip : Com
+    | Asgn : Loc -> AExp -> Com
+    | Seq : Com -> Com -> Com
+    | If : BExp -> Com -> Com -> Com
+    | While : BExp -> Com -> Com.
+
+Definition State : Type := Loc -> nat.
+
+Definition initialState : State := fun _ => 0.
+
+Definition changeState (s : State) (x : Loc) (n : nat) : State :=
+  fun y : Loc => if x =? y then n else s y.
+
+Fixpoint aeval (s : State) (a : AExp) : nat :=
+match a with
+    | AConst n => n
+    | Var v => s v
+    | ABinOp f a1 a2 => f (aeval s a1) (aeval s a2)
+end.
+
+Fixpoint loca (a : AExp) : list Loc :=
+match a with
+    | AConst _ => []
+    | Var x => [x]
+    | ABinOp f a1 a2 => loca a1 ++ loca a2
+end.
+
+Definition acompatible (a : AExp) (s1 s2 : State) : Prop :=
+  forall x : Loc, In x (loca a) -> s1 x = s2 x.
+
+Fixpoint beval (s : State) (e : BExp) : bool :=
+match e with
+    | BConst b => b
+    | BRelOp f a1 a2 => f (aeval s a1) (aeval s a2)
+    | Not e' => negb (beval s e')
+    | BBinOp f e1 e2 => f (beval s e1) (beval s e2)
+end.
+
+Fixpoint locb (b : BExp) : list Loc :=
+match b with
+    | BConst _ => []
+    | BRelOp _ a1 a2 => loca a1 ++ loca a2
+    | Not b' => locb b'
+    | BBinOp _ b1 b2 => locb b1 ++ locb b2
+end.
+
+Definition bcompatible (b : BExp) (s1 s2 : State) : Prop :=
+  forall x : Loc, In x (locb b) -> s1 x = s2 x.
+
+Function ceval (n : nat) (c : Com) (s : State) : option State :=
+match n with
+    | 0 => None
+    | S n' =>
+        match c with
+            | Skip => Some s
+            | Asgn x a => Some (changeState s x (aeval s a))
+            | Seq c1 c2 =>
+                match ceval n' c1 s with
+                    | None => None
+                    | Some s' => ceval n' c2 s'
+                end
+            | If b c1 c2 =>
+                if beval s b then ceval n' c1 s else ceval n' c2 s
+            | While b c =>
+                if beval s b
+                then
+                  match ceval n' c s with
+                      | None => None
+                      | Some s' => ceval n' (While b c) s'
+                  end
+                else Some s
+        end
+end.
+
+(* The list of all variables which are assigned to by the instruction c. *)
+Fixpoint locw (c : Com) : list Loc :=
+match c with
+    | Skip => []
+    | Asgn v _ => [v]
+    | Seq c1 c2 => locw c1 ++ locw c2
+    | If _ c1 c2 => locw c1 ++ locw c2
+    | While _ c => locw c
+end.
+
+Definition wcompatible (c : Com) (s1 s2 : State) : Prop :=
+  forall x : Loc, In x (locw c) -> s1 x = s2 x.
+
+(* The list of all variables mentioned in c. *)
+Fixpoint loc (c : Com) : list Loc :=
+match c with
+    | Skip => []
+    | Asgn v a => v :: loca a
+    | Seq c1 c2 => loc c1 ++ loc c2
+    | If b c1 c2 => locb b ++ loc c1 ++ loc c2
+    | While b c => locb b ++ loc c
+end.
+
+Definition ccompatible (c : Com) (s1 s2 : State) : Prop :=
+  forall x : Loc, In x (loc c) -> s1 x = s2 x.
