Imps/Imp/Imp_BigStep.v
@@ -1,0 +1,558 @@
+Add Rec LoadPath "~/Code/Coq".
+
+Require Import ImpSyntax.
+
+Inductive AEval : AExp -> State -> nat -> Prop :=
+    | EvalAConst :
+        forall (n : nat) (s : State), AEval (AConst n) s n
+    | EvalVar :
+        forall (v : Loc) (s : State), AEval (Var v) s (s v)
+    | EvalABinOp :
+        forall (f : nat -> nat -> nat)
+               (a1 a2 : AExp) (s : State) (n1 n2 : nat),
+          AEval a1 s n1 -> AEval a2 s n2 ->
+            AEval (ABinOp f a1 a2) s (f n1 n2).
+
+Hint Constructors AEval.
+
+Lemma AEval_aeval :
+  forall {a : AExp} {s : State} {n : nat},
+    AEval a s n -> aeval s a = n.
+Proof.
+  induction 1; cbn; rewrite ?IHAEval1, ?IHAEval2; reflexivity.
+Qed.
+
+Lemma aeval_AEval :
+  forall {a : AExp} {s : State} {n : nat},
+    aeval s a = n -> AEval a s n.
+Proof.
+  induction a; cbn; intros; rewrite <- H; auto.
+Defined.
+
+Lemma AEval_det :
+  forall {a : AExp} {s : State} {n m : nat},
+    AEval a s n -> AEval a s m -> n = m.
+Proof.
+  intros a s n m H. revert m.
+  induction H; inversion 1; subst; clear H.
+    1-2: reflexivity.
+    rewrite (IHAEval1 _ H7), (IHAEval2 _ H8). reflexivity.
+Restart.
+  intros.
+  apply AEval_aeval in H.
+  apply AEval_aeval in H0.
+  rewrite <- H, <- H0.
+  reflexivity.
+Qed.
+
+Lemma AEval_acompatible :
+  forall {a : AExp} {s1 : State} {n : nat},
+    AEval a s1 n -> forall {s2 : State},
+      acompatible a s1 s2 ->
+        AEval a s2 n.
+Proof.
+  Hint Resolve in_or_app.
+  unfold acompatible.
+  induction 1; cbn in *; intros; try rewrite H; auto 6.
+Qed.
+
+Lemma AEval_acompatible_det :
+  forall {a : AExp} {s1 : State} {n1 : nat},
+    AEval a s1 n1 ->
+    forall {s2 : State} {n2 : nat},
+      AEval a s2 n2 ->
+      (forall x : Loc, In x (loca a) -> s1 x = s2 x) ->
+        n1 = n2.
+Proof.
+  induction 1; cbn; intros; auto.
+    inv H. reflexivity.
+    inv H. apply H0. left. reflexivity.
+    inv H1. erewrite IHAEval1, IHAEval2; eauto.
+Qed.
+
+Inductive BEval : BExp -> State -> bool -> Prop :=
+    | EvalBConst :
+        forall (s : State) (b : bool), BEval (BConst b) s b
+    | BEval_BRelOp :
+        forall (f : nat -> nat -> bool)
+               (a1 a2 : AExp) (s : State) (n1 n2 : nat),
+          AEval a1 s n1 -> AEval a2 s n2 ->
+            BEval (BRelOp f a1 a2) s (f n1 n2)
+    | EvalNot :
+        forall (e : BExp) (s : State) (b : bool),
+          BEval e s b -> BEval (Not e) s (negb b)
+    | BEval_BBinOp :
+        forall (f : bool -> bool -> bool)
+               (e1 e2 : BExp) (s : State) (b1 b2 : bool),
+          BEval e1 s b1 -> BEval e2 s b2 ->
+            BEval (BBinOp f e1 e2) s (f b1 b2).
+
+Hint Constructors BEval.
+
+Lemma BEval_beval :
+  forall {e : BExp} {s : State} {b : bool},
+    BEval e s b -> beval s e = b.
+Proof.
+  induction 1; cbn.
+    reflexivity.
+    rewrite (AEval_aeval H), (AEval_aeval H0). reflexivity.
+    rewrite IHBEval. reflexivity.
+    rewrite IHBEval1, IHBEval2. reflexivity.
+Qed.
+
+Lemma beval_BEval :
+  forall {e : BExp} {s : State} {b : bool},
+    beval s e = b -> BEval e s b.
+Proof.
+  induction e; cbn; intros; subst; auto.
+    constructor; apply aeval_AEval; reflexivity.
+Qed.
+
+Lemma BEval_det :
+  forall {e : BExp} {s : State} {b1 : bool},
+    BEval e s b1 -> forall {b2 : bool}, BEval e s b2 -> b1 = b2.
+Proof.
+  induction 1; intros.
+    inv H. reflexivity.
+    inv H1. rewrite (AEval_det H H7), (AEval_det H0 H8). reflexivity.
+    inv H0. rewrite (IHBEval _ H2). reflexivity.
+    inv H1. rewrite (IHBEval1 _ H7), (IHBEval2 _ H8). reflexivity.
+Restart.
+  intros.
+  apply BEval_beval in H.
+  apply BEval_beval in H0.
+  rewrite <- H, <- H0.
+  reflexivity.
+Qed.
+
+Lemma BEval_bcompatible :
+  forall {e : BExp} {s1 : State} {b : bool},
+    BEval e s1 b -> forall {s2 : State},
+      bcompatible e s1 s2 -> BEval e s2 b.
+Proof.
+  Hint Resolve AEval_acompatible.
+  Hint Unfold acompatible.
+  unfold bcompatible.
+  induction 1; cbn in *; intros; constructor; eauto 6.
+Qed.
+
+Lemma BEval_bcompatible_det :
+  forall {e : BExp} {s1 : State} {b1 : bool},
+    BEval e s1 b1 -> forall {s2 : State} {b2 : bool},
+    BEval e s2 b2 ->
+      bcompatible e s1 s2 -> b1 = b2.
+Proof.
+  intros.
+  assert (BEval e s2 b1).
+    eapply BEval_bcompatible; eauto.
+  eapply BEval_det; eauto.
+Qed.
+
+Inductive CEval : Com -> State -> State -> Prop :=
+    | EvalSkip :
+        forall s : State, CEval Skip s s
+    | EvalAsgn :
+        forall (v : Loc) (a : AExp) (s : State) (n : nat),
+          AEval a s n -> CEval (Asgn v a) s (changeState s v n)
+    | EvalSeq :
+        forall (c1 c2 : Com) (s1 s2 s3 : State),
+          CEval c1 s1 s2 -> CEval c2 s2 s3 -> CEval (Seq c1 c2) s1 s3
+    | EvalIfFalse :
+        forall (b : BExp) (c1 c2 : Com) (s1 s2 : State),
+          BEval b s1 false -> CEval c2 s1 s2 -> CEval (If b c1 c2) s1 s2
+    | EvalIfTrue :
+        forall (b : BExp) (c1 c2 : Com) (s1 s2 : State),
+          BEval b s1 true -> CEval c1 s1 s2 -> CEval (If b c1 c2) s1 s2
+    | EvalWhileFalse :
+        forall (b : BExp) (c : Com) (s : State),
+          BEval b s false -> CEval (While b c) s s
+    | EvalWhileTrue :
+        forall (b : BExp) (c : Com) (s1 s2 s3 : State),
+          BEval b s1 true ->
+          CEval c s1 s2 -> CEval (While b c) s2 s3 ->
+            CEval (While b c) s1 s3.
+
+Hint Constructors CEval.
+
+Lemma CEval_det :
+  forall (c : Com) (s s1 : State),
+    CEval c s s1 -> forall s2 : State, CEval c s s2 -> s1 = s2.
+Proof.
+  induction 1; intros.
+    inv H. reflexivity.
+    inv H0. rewrite (AEval_det H H5). reflexivity.
+    inv H1. specialize (IHCEval1 _ H4). subst.
+      specialize (IHCEval2 _ H7). subst. reflexivity.
+    inv H1.
+      rewrite (IHCEval _ H8). reflexivity.
+      pose (BEval_det H H7). congruence.
+    inv H1.
+      pose (BEval_det H H7). congruence.
+      rewrite (IHCEval _ H8). reflexivity.
+    inv H0.
+      reflexivity.
+      pose (BEval_det H H3). congruence.
+    inv H2.
+      pose (BEval_det H H7). congruence.
+      specialize (IHCEval1 _ H6). subst.
+        specialize (IHCEval2 _ H9). subst. reflexivity.
+Restart.
+  Hint Rewrite @AEval_det.
+  Hint Resolve AEval_det BEval_det.
+  induction 1; intros.
+  Ltac wut :=
+  match goal with
+      | H : CEval ?c _ _ |- _ => is_var c + inv H
+  end;
+  repeat match goal with
+      | IH : forall _, CEval _ _ _ -> _, H : CEval _ _ _ |- _ =>
+          let H' := fresh "H" in
+            assert (H' := IH _ H); clear H; rename H' into H; subst
+      | H : BEval ?b ?s _, H' : BEval ?b ?s _ |- _ =>
+          let H'' := fresh "H" in
+            assert (H'' := BEval_det H H'); clear H H'
+  end; eauto; try congruence.
+  all: wut.
+Qed.
+
+Hint Immediate aeval_AEval beval_BEval.
+
+Lemma ceval_CEval :
+  forall (n : nat) (c : Com) (s1 s2 : State),
+    ceval n c s1 = Some s2 -> CEval c s1 s2.
+Proof.
+  intros n c s1. functional induction ceval n c s1; intros; inv H; eauto.
+Qed.
+
+Lemma ceval_plus :
+  forall (n k : nat) (c : Com) (s1 s2 : State),
+    ceval n c s1 = Some s2 -> ceval (n + k) c s1 = Some s2.
+Proof.
+  induction n as [| n']; cbn; intros.
+    inv H.
+    destruct c; auto.
+      destruct (ceval n' c1 s1) eqn: Heq.
+        erewrite IHn'; eauto.
+        inv H.
+      destruct (beval s1 b) eqn: Hb; eauto.
+      destruct (beval s1 b) eqn: Hb; eauto.
+        destruct (ceval n' c s1) eqn: Heq.
+          erewrite IHn'; eauto.
+          inv H.
+Qed.
+
+Lemma CEval_ceval :
+  forall (c : Com) (s1 s2 : State),
+    CEval c s1 s2 -> exists n : nat, ceval n c s1 = Some s2.
+Proof.
+  induction 1.
+    exists 1. cbn. reflexivity.
+    exists 1. cbn. do 2 f_equal. apply AEval_aeval. assumption.
+    destruct IHCEval1 as [n1 IH1], IHCEval2 as [n2 IH2].
+      exists (S (n1 + n2)). (* Should be S (max n1 n2) *)
+      cbn. rewrite (ceval_plus n1 n2 _ _ _ IH1), plus_comm.
+        apply ceval_plus. assumption.
+    destruct IHCEval as [n IH]. exists (S n). cbn.
+      apply BEval_beval in H. rewrite H. assumption.
+    destruct IHCEval as [n IH]. exists (S n). cbn.
+      apply BEval_beval in H. rewrite H. assumption.
+    exists 1. cbn. apply BEval_beval in H. rewrite H. reflexivity.
+    destruct IHCEval1 as [n1 IH1], IHCEval2 as [n2 IH2].
+      exists (S (n1 + n2)). cbn. (* Should be S (max n1 n2) *)
+      apply BEval_beval in H. rewrite H.
+      rewrite (ceval_plus _ _ _ _ _ IH1), plus_comm.
+      apply ceval_plus. assumption.
+Qed.
+
+Lemma while_true_do_skip :
+  forall s1 s2 : State,
+    ~ CEval (While (BConst true) Skip) s1 s2.
+Proof.
+  intros s1 s2 H.
+  remember (While (BConst true) Skip) as w. revert Heqw.
+  induction H; intros; inv Heqw.
+    inv H.
+    apply IHCEval2. reflexivity.
+Qed.
+
+Lemma CEval_not_In_locw_eq :
+  forall (c : Com) (s1 s2 : State),
+    CEval c s1 s2 -> forall x : Loc, ~ In x (locw c) -> s1 x = s2 x.
+Proof.
+  induction 1; cbn in *; intros; auto.
+    unfold changeState. destruct (dec_spec v x).
+      subst. contradiction H0. left. reflexivity.
+      reflexivity.
+    all: rewrite ?IHCEval, ?IHCEval1, ?IHCEval2; auto.
+Qed.
+
+Lemma CEval_not_In_loc_eq :
+  forall (c : Com) (s1 s2 : State),
+    CEval c s1 s2 -> forall x : Loc, ~ In x (loc c) -> s1 x = s2 x.
+Proof.
+  induction 1; cbn in *; intros; auto.
+    unfold changeState. destruct (dec_spec v x).
+      subst. contradiction H0. left. reflexivity.
+      reflexivity.
+    all: rewrite ?IHCEval, ?IHCEval1, ?IHCEval2; auto 7.
+Qed.
+
+Lemma CEval_ccompatible :
+  forall (c : Com) (s1 s2 : State),
+    CEval c s1 s2 ->
+    forall {s1' s2' : State},
+      CEval c s1' s2' ->
+        ccompatible c s1 s1' -> ccompatible c s2 s2'.
+Proof.
+  unfold ccompatible.
+  Hint Unfold bcompatible.
+  induction 1; cbn; intros.
+    inv H1.
+    inv H0. unfold changeState. inv H2.
+      destruct (dec_spec x x).
+        eapply AEval_acompatible_det; eauto.
+        contradiction.
+      destruct (dec_spec v x).
+        eapply AEval_acompatible_det; eauto.
+        auto.
+    Focus 4. inv H0.
+      apply H1. assumption.
+      assert (false = true).
+        eapply BEval_bcompatible_det; eauto. congruence.
+(* If *)
+(*
+    Focus 2. inv H1.
+      eapply IHCEval; eauto 6.
+*)
+(* Seq *)
+(*
+    inv H1. apply in_app_or in H3. destruct H3.
+      assert (In x (loc c2) \/ ~ In x (loc c2)).
+        admit.
+        destruct H3.
+          assert (ccompatible c1 s2 s4).
+            red. intros. eapply IHCEval1; eauto.
+            red in H4. eapply IHCEval2; eauto. intros.
+              apply H4. assumption.
+*)
+(* While *)
+(*
+    Focus 4. inv H2; cbn in *.
+      assert (false = true); try congruence.
+        eapply BEval_bcompatible_det; eauto. unfold bcompatible.
+          intros. symmetry. auto.
+      assert (s1 x = s1' x).
+        apply H3. assumption.
+        assert (s3 x = s2' x).
+          eapply IHCEval2; eauto. intros. apply in_app_or in H5. inv H5.
+*)
+Abort.
+
+(* Program equivalence. *)
+
+Definition equivalent (c1 c2 : Com) : Prop :=
+  forall s1 s2 : State,
+    CEval c1 s1 s2 <-> CEval c2 s1 s2.
+
+Notation "c1 ~ c2" := (equivalent c1 c2) (at level 50).
+
+Example equivalent_ex1 :
+  forall (b : BExp) (c : Com),
+    While b c ~ If b (Seq c (While b c)) Skip.
+Proof.
+  unfold equivalent. split; intros.
+    remember (While b c) as w. revert b c Heqw.
+      induction H; intros; inv Heqw; eauto.
+    inv H; inv H6; eauto.
+Defined.
+
+(* TODO: for loop *)
+
+Inductive Context : Type :=
+    | CContext : Context
+    | CSeqL : Context -> Com -> Context
+    | CSeqR : Com -> Context -> Context
+    | CIfL : BExp -> Context -> Com -> Context
+    | CIfR : BExp -> Com -> Context -> Context
+    | CWhile : BExp -> Context -> Context.
+
+Fixpoint put (G : Context) (c : Com) : Com :=
+match G with
+    | CContext => c
+    | CSeqL G' c' => Seq (put G' c) c'
+    | CSeqR c' G' => Seq c' (put G' c)
+    | CIfL b G' c' => If b (put G' c) c'
+    | CIfR b c' G' => If b c' (put G' c)
+    | CWhile b G' => While b (put G' c)
+end.
+
+Lemma equivalent_in_Context :
+  forall c1 c2 : Com,
+    c1 ~ c2 -> forall G : Context, put G c1 ~ put G c2.
+Proof.
+  intros c1 c2 H G. revert c1 c2 H.
+  induction G; cbn; intros.
+    assumption.
+    all: unfold equivalent in *; split; intros.
+      inv H0. econstructor.
+        rewrite IHG; eauto. firstorder.
+        assumption.
+      inv H0. econstructor; rewrite 1?IHG; eauto.
+      inv H0. econstructor; rewrite 1?IHG; eauto. firstorder.
+      inv H0. econstructor; rewrite 1?IHG; eauto.
+      inv H0.
+        econstructor; rewrite 1?IHG; eauto.
+        apply EvalIfTrue; eauto. rewrite IHG; eauto. firstorder.
+      inv H0.
+        econstructor; rewrite 1?IHG; eauto.
+        apply EvalIfTrue; eauto. rewrite IHG; eauto.
+      inv H0.
+        econstructor; rewrite 1?IHG; eauto. firstorder.
+        apply EvalIfTrue; eauto.
+      inv H0.
+        econstructor; rewrite 1?IHG; eauto.
+        firstorder.
+      remember (While b (put G c1)) as w. revert Heqw.
+      induction H0; intro; inv Heqw.
+        eauto.
+        econstructor; eauto. rewrite IHG; eauto. firstorder.
+      remember (While b (put G c2)) as w. revert Heqw.
+      induction H0; intro; inv Heqw.
+        eauto.
+        econstructor; eauto. rewrite IHG; eauto.
+Restart.
+  intros c1 c2 H G. revert c1 c2 H.
+  induction G; cbn; intros; eauto;
+  unfold equivalent in *; split; intros;
+  match goal with
+      | H : CEval ?c _ _ |- _ =>
+          let c' := fresh "c" in
+          let Heqc' := fresh "Heq" c' in
+            remember c as c'; revert Heqc';
+            induction H; intros; inv Heqc'
+  end; eauto.
+    5-6: apply EvalIfTrue; rewrite 1?IHG; eauto; firstorder.
+    all: econstructor; rewrite 1?IHG; eauto; firstorder.
+Qed.
+
+(** [equivalent] is a congruence *)
+
+Lemma equivalent_Seq_l :
+  forall c c1 c2 : Com,
+    c1 ~ c2 -> Seq c1 c ~ Seq c2 c.
+Proof.
+  unfold equivalent. split; intros.
+    inv H0. econstructor.
+      rewrite <- H. eassumption.
+      assumption.
+    inv H0. econstructor.
+      rewrite H. eassumption.
+      assumption.
+Qed.
+
+Lemma equivalent_Seq_r :
+  forall c c1 c2 : Com,
+    c1 ~ c2 -> Seq c c1 ~ Seq c c2.
+Proof.
+  unfold equivalent. split; intros.
+    inv H0. econstructor.
+      eassumption.
+      rewrite <- H. eassumption.
+    inv H0. econstructor.
+      eassumption.
+      rewrite H. eassumption.
+Qed.
+
+Lemma equivalent_If_l :
+  forall (b : BExp) (c c1 c2 : Com),
+    c1 ~ c2 -> If b c1 c ~ If b c2 c.
+Proof.
+  unfold equivalent. split; intros.
+    inv H0.
+      constructor; assumption.
+      apply EvalIfTrue.
+        assumption.
+        rewrite <- H. assumption.
+    inv H0.
+      constructor; assumption.
+      apply EvalIfTrue.
+        assumption.
+        rewrite H. assumption.
+Qed.
+
+Lemma equivalent_If_r :
+  forall (b : BExp) (c c1 c2 : Com),
+    c1 ~ c2 -> If b c c1 ~ If b c c2.
+Proof.
+  unfold equivalent. split; intros.
+    inv H0.
+      constructor.
+        assumption.
+        rewrite <- H. assumption.
+      apply EvalIfTrue; assumption.
+    inv H0.
+      constructor.
+        assumption.
+        rewrite H. assumption.
+      apply EvalIfTrue; assumption.
+Qed.
+
+Lemma equivalent_While :
+  forall (b : BExp) (c c1 c2 : Com),
+    c1 ~ c2 -> While b c1 ~ While b c2.
+Proof.
+  unfold equivalent. split; intros.
+    remember (While b c1) as w. revert Heqw. induction H0; intro; inv Heqw.
+      constructor. assumption.
+      eapply EvalWhileTrue.
+        assumption.
+        rewrite <- H. eassumption.
+        apply IHCEval2. reflexivity.
+    remember (While b c2) as w. revert Heqw. induction H0; intro; inv Heqw.
+      constructor. assumption.
+      eapply EvalWhileTrue.
+        assumption.
+        rewrite H. eassumption.
+        apply IHCEval2. reflexivity.
+Qed.
+
+(** * Observational equivalence *)
+
+Definition Observation (A : Type) : Type := Com -> A.
+
+Definition oequiv {A : Type} (c1 c2 : Com) : Prop :=
+  forall (G : Context) (f : Observation A),
+    f (put G c1) = f (put G c2).
+
+(** * Nontermination *)
+
+CoInductive NonTerm : Com -> State -> Prop :=
+    | NT_SeqL :
+        forall (c1 c2 : Com) (s : State),
+          NonTerm c1 s -> NonTerm (Seq c1 c2) s
+    | NT_SeqR :
+        forall (c1 c2 : Com) (s1 s2 : State),
+          CEval c1 s1 s2 -> NonTerm c2 s2 -> NonTerm (Seq c1 c2) s1
+    | NT_IfTrue :
+        forall (b : BExp) (c1 c2 : Com) (s : State),
+          BEval b s true -> NonTerm c1 s -> NonTerm (If b c1 c2) s
+    | NT_IfFalse :
+        forall (b : BExp) (c1 c2 : Com) (s : State),
+          BEval b s false -> NonTerm c2 s -> NonTerm (If b c1 c2) s
+    | NT_WhileBody :
+        forall (b : BExp) (c : Com) (s : State),
+          BEval b s true -> NonTerm c s -> NonTerm (While b c) s
+    | NT_WhileSelf :
+        forall (b : BExp) (c : Com) (s1 s2 : State),
+          BEval b s1 true -> CEval c s1 s2 -> NonTerm (While b c) s2 ->
+            NonTerm (While b c) s1.
+
+Lemma NT_While_true_do_Skip :
+  forall s : State,
+    NonTerm (While (BConst true) Skip) s.
+Proof.
+  intro. cofix IH. eapply NT_WhileSelf.
+    auto.
+    auto.
+    assumption.
+Qed.
