Imps/Imp/Imp_SmallStep_Context.v
@@ -1,0 +1,83 @@
+Add Rec LoadPath "~/Code/Coq".
+
+Require Import ImpSyntax.
+
+(** * Structural operational semantics for IMP using contexts *)
+
+Inductive AStep (s : State) : AExp -> AExp -> Prop :=
+    | AStep_Var :
+        forall x : Loc, AStep s (Var x) (AConst (s x))
+    | AStep_ABinOp :
+        forall (f : nat -> nat -> nat) (n1 n2 : nat),
+          AStep s (ABinOp f (AConst n1) (AConst n2)) (AConst (f n1 n2)).
+
+Inductive AContext : Type :=
+    | AC_Var : AContext
+    | AC_L : (nat -> nat -> nat) -> AContext -> AExp -> AContext
+    | AC_R : (nat -> nat -> nat) -> nat -> AContext -> AContext.
+
+Fixpoint put (G : AContext) (a : AExp) : AExp :=
+match G with
+    | AC_Var => a
+    | AC_L f G' a' => ABinOp f (put G' a) a'
+    | AC_R f n G' => ABinOp f (AConst n) (put G' a)
+end.
+
+Inductive AEval (s : State) : AExp -> AExp -> Prop :=
+    | AEval_put :
+        forall (a1 a2 : AExp) (G : AContext),
+          AStep s a1 a2 -> AEval s (put G a1) (put G a2).
+
+Hint Constructors AStep AEval.
+
+Require Import Recdef.
+
+Function AExp_to_AContext (a : AExp) : AContext * AExp :=
+match a with
+    | AConst n => (AC_Var, AConst n)
+    | Var x => (AC_Var, Var x)
+    | ABinOp f (AConst n) a2 =>
+        let '(G, a) := AExp_to_AContext a2 in (AC_R f n G, a)
+    | ABinOp f a1 a2 =>
+        let '(G, a) := AExp_to_AContext a1 in (AC_L f G a2, a)
+end.
+
+Lemma AExp_to_AContext_put :
+  forall (a1 a2 : AExp) (G : AContext),
+    AExp_to_AContext a1 = (G, a2) -> put G a2 = a1.
+Proof.
+  intros a1.
+  functional induction AExp_to_AContext a1;
+    intros; inv H; cbn; f_equal; auto.
+Qed.
+
+Lemma AExp_to_AContext_put' :
+  forall a : AExp,
+    put (fst (AExp_to_AContext a)) (snd (AExp_to_AContext a)) = a.
+Proof.
+  intros. apply AExp_to_AContext_put.
+  destruct AExp_to_AContext. cbn. reflexivity.
+Qed.
+
+Require Imp.Imp_SmallStep.
+
+Lemma AEval_AEval :
+  forall (s : State) (a1 a2 : AExp),
+    AEval s a1 a2 <-> Imp_SmallStep.AEval s a1 a2.
+Proof.
+  split.
+    intro. inv H. induction G; cbn; auto. induction H0; auto.
+    rewrite <- (AExp_to_AContext_put' a1) at 2.
+    rewrite <- (AExp_to_AContext_put' a2) at 2.
+    induction 1.
+      constructor; cbn; auto.
+Admitted.
+(*
+apply AExp_to_AContext_put in x.
+ destruct x as [G1 a1'].
+    pose (x := AExp_to_AContext a2). destruct x as [G2 a2'].
+    
+    induction 1.
+      change (Var x) with (put ACVar (Var x)).
+      change (AConst (s x)) with (put ACVar (AConst (s x))). auto.
+*)
