Imps/Imp_resultis.v
@@ -1,0 +1,256 @@
+Add LoadPath "~/Code/Coq".
+
+Require Import FormalSystems.Base.
+
+Inductive AExp : Type :=
+    | AConst : nat -> AExp
+    | Var : Loc -> AExp
+    | Add : AExp -> AExp -> AExp
+    | Sub : AExp -> AExp -> AExp
+    | Mul : AExp -> AExp -> AExp
+    | ResultIs : Com -> AExp -> AExp
+
+with BExp : Type :=
+    | BTrue : BExp
+    | BFalse : BExp
+    | Eq : AExp -> AExp -> BExp
+    | Le : AExp -> AExp -> BExp
+    | Not : BExp -> BExp
+    | And : BExp -> BExp -> BExp
+    | Or : BExp -> BExp -> BExp
+
+with Com : Type :=
+    | Skip : Com
+    | Asgn : Loc -> AExp -> Com
+    | Seq : Com -> Com -> Com
+    | If : BExp -> Com -> Com -> Com
+    | While : BExp -> Com -> Com.
+
+Definition State : Type := Loc -> nat.
+
+Definition initialState : State := fun _ => 0.
+
+Definition changeState (s : State) (x : Loc) (n : nat) : State :=
+  fun y : Loc => if x =? y then n else s y.
+
+Inductive AEval : AExp -> State -> nat -> Prop :=
+    | EvalAConst :
+        forall (n : nat) (s : State), AEval (AConst n) s n
+    | EvalVar :
+        forall (v : Loc) (s : State), AEval (Var v) s (s v)
+    | EvalAdd :
+        forall (a1 a2 : AExp) (s : State) (n1 n2 : nat),
+          AEval a1 s n1 -> AEval a2 s n2 -> AEval (Add a1 a2) s (n1 + n2)
+    | EvalSub :
+        forall (a1 a2 : AExp) (s : State) (n1 n2 : nat),
+          AEval a1 s n1 -> AEval a2 s n2 -> AEval (Sub a1 a2) s (n1 - n2)
+    | EvalMul :
+        forall (a1 a2 : AExp) (s : State) (n1 n2 : nat),
+          AEval a1 s n1 -> AEval a2 s n2 -> AEval (Mul a1 a2) s (n1 * n2)
+    | EvalResultIs :
+        forall (c : Com) (a : AExp) (s1 s2 : State) (n : nat),
+          CEval c s1 s2 -> AEval a s2 n -> AEval (ResultIs c a) s1 n
+
+with BEval : BExp -> State -> bool -> Prop :=
+    | EvalTrue :
+        forall s : State, BEval BTrue s true
+    | EvalFalse :
+        forall s : State, BEval BFalse s false
+    | EvalEq :
+        forall (a1 a2 : AExp) (s : State) (n m : nat),
+          AEval a1 s n -> AEval a2 s m -> BEval (Eq a1 a2) s (Nat.eqb n m)
+    | EvalLe :
+        forall (a1 a2 : AExp) (s : State) (n m : nat),
+          AEval a1 s n -> AEval a2 s m -> BEval (Le a1 a2) s (Nat.leb n m)
+    | EvalNot :
+        forall (e : BExp) (s : State) (b : bool),
+          BEval e s b -> BEval (Not e) s (negb b)
+    | EvalAnd :
+        forall (e1 e2 : BExp) (s : State) (b1 b2 : bool),
+          BEval e1 s b1 -> BEval e2 s b2 -> BEval (And e1 e2) s (andb b1 b2)
+    | EvalOr :
+        forall (e1 e2 : BExp) (s : State) (b1 b2 : bool),
+          BEval e1 s b1 -> BEval e2 s b2 -> BEval (Or e1 e2) s (orb b1 b2)
+
+with CEval : Com -> State -> State -> Prop :=
+    | EvalSkip :
+        forall s : State, CEval Skip s s
+    | EvalAsgn :
+        forall (v : Loc) (a : AExp) (s : State) (n : nat),
+          AEval a s n -> CEval (Asgn v a) s (changeState s v n)
+    | EvalSeq :
+        forall (c1 c2 : Com) (s1 s2 s3 : State),
+          CEval c1 s1 s2 -> CEval c2 s2 s3 -> CEval (Seq c1 c2) s1 s3
+    | EvalIfFalse :
+        forall (b : BExp) (c1 c2 : Com) (s1 s2 : State),
+          BEval b s1 false -> CEval c2 s1 s2 -> CEval (If b c1 c2) s1 s2
+    | EvalIfTrue :
+        forall (b : BExp) (c1 c2 : Com) (s1 s2 : State),
+          BEval b s1 true -> CEval c1 s1 s2 -> CEval (If b c1 c2) s1 s2
+    | EvalWhileFalse :
+        forall (b : BExp) (c : Com) (s : State),
+          BEval b s false -> CEval (While b c) s s
+    | EvalWhileTrue :
+        forall (b : BExp) (c : Com) (s1 s2 s3 : State),
+          BEval b s1 true ->
+          CEval c s1 s2 -> CEval (While b c) s2 s3 ->
+            CEval (While b c) s1 s3.
+
+Hint Constructors AEval BEval CEval.
+
+Ltac inv H :=
+  inversion H; subst; clear H; auto.
+
+Lemma AEval_det :
+  forall {a : AExp} {s : State} {n m : nat},
+    AEval a s n -> AEval a s m -> n = m
+
+with BEval_det :
+  forall {e : BExp} {s : State} {b1 : bool},
+    BEval e s b1 -> forall {b2 : bool}, BEval e s b2 -> b1 = b2
+
+with CEval_det :
+  forall (c : Com) (s s1 : State),
+    CEval c s s1 -> forall s2 : State, CEval c s s2 -> s1 = s2.
+Proof.
+  destruct 1; intros * HI *; inv HI.
+    rewrite (AEval_det _ _ _ _ H H3), (AEval_det _ _ _ _ H0 H6). reflexivity.
+    rewrite (AEval_det _ _ _ _ H H3), (AEval_det _ _ _ _ H0 H6). reflexivity.
+    rewrite (AEval_det _ _ _ _ H H3), (AEval_det _ _ _ _ H0 H6). reflexivity.
+    specialize (CEval_det _ _ _ H _ H3). subst.
+      rewrite (AEval_det _ _ _ _ H0 H6). reflexivity.
+  destruct 1; intros * HI *; inv HI.
+    rewrite (AEval_det _ _ _ _ H H3), (AEval_det _ _ _ _ H0 H6). reflexivity.
+    rewrite (AEval_det _ _ _ _ H H3), (AEval_det _ _ _ _ H0 H6). reflexivity.
+    rewrite (BEval_det _ _ _ H _ H1). reflexivity.
+    rewrite (BEval_det _ _ _ H _ H3), (BEval_det _ _ _ H0 _ H6). reflexivity.
+    rewrite (BEval_det _ _ _ H _ H3), (BEval_det _ _ _ H0 _ H6). reflexivity.
+  destruct 1; intros * HI *; inv HI.
+    rewrite (AEval_det _ _ _ _ H H4). reflexivity.
+    destruct (CEval_det _ _ _ H _ H3), (CEval_det _ _ _ H0 _ H6). reflexivity.
+    rewrite (CEval_det _ _ _ H0 _ H7). reflexivity.
+    specialize (BEval_det _ _ _ H _ H6). congruence.
+    specialize (BEval_det _ _ _ H _ H6). congruence.
+    rewrite (CEval_det _ _ _ H0 _ H7). reflexivity.
+    specialize (BEval_det _ _ _ H _ H2). congruence.
+    specialize (BEval_det _ _ _ H _ H6). congruence.
+    destruct (CEval_det _ _ _ H0 _ H5), (CEval_det _ _ _ H1 _ H8). reflexivity.
+Qed.
+
+Require Import Recdef.
+
+Function aeval (n : nat) (a : AExp) (s : State) : option nat := 
+match n with
+  | 0 => None
+  | S n' =>
+      match a with
+        | AConst n => Some n
+        | Var v => Some (s v)
+        | Add a1 a2 => liftM2 plus (aeval n' a1 s) (aeval n' a2 s)
+        | Sub a1 a2 => liftM2 minus (aeval n' a1 s) (aeval n' a2 s)
+        | Mul a1 a2 => liftM2 mult (aeval n' a1 s) (aeval n' a2 s)
+        | ResultIs c a' =>
+            match ceval n' c s with
+                | None => None
+                | Some s' => aeval n' a' s'
+            end
+      end
+end
+
+with beval (n : nat) (e : BExp) (s : State) : option bool :=
+match n with
+  | 0 => None
+  | S n' =>
+      match e with
+        | BTrue => Some true
+        | BFalse => Some false
+        | Eq a1 a2 => liftM2 Nat.eqb (aeval n' a1 s) (aeval n' a2 s)
+        | Le a1 a2 => liftM2 Nat.leb (aeval n' a1 s) (aeval n' a2 s)
+        | Not e' => omap negb (beval n' e' s)
+        | And e1 e2 => liftM2 andb (beval n' e1 s) (beval n' e2 s)
+        | Or e1 e2 => liftM2 orb (beval n' e1 s) (beval n' e2 s)
+      end
+end
+
+with ceval (n : nat) (c : Com) (s : State) : option State :=
+match n with
+  | 0 => None
+  | S n' =>
+      match c with
+        | Skip => Some s
+        | Asgn x a => omap (changeState s x) (aeval n' a s)
+        | Seq c1 c2 => obind (ceval n' c1 s) (ceval n' c2)
+        | If b c1 c2 =>
+            match beval n' b s with
+                | None => None
+                | Some true => ceval n' c1 s
+                | Some false => ceval n' c2 s
+            end
+        | While b c =>
+            match beval n' b s with
+                | None => None
+                | Some true => obind (ceval n' c s) (ceval n' (While b c))
+                | Some false => Some s
+            end
+      end
+end.
+
+Fixpoint aeval_AEval (fuel : nat) :
+  forall {a : AExp} {s : State} {n : nat},
+    aeval fuel a s = Some n -> AEval a s n
+
+with beval_BEval (fuel : nat) :
+  forall {e : BExp} {s : State} {b : bool},
+    beval fuel e s = Some b -> BEval e s b
+
+with ceval_CEval (fuel : nat) :
+  forall {c : Com} {s1 s2 : State},
+    ceval fuel c s1 = Some s2 -> CEval c s1 s2.
+Proof.
+  destruct fuel as [| fuel']; cbn; intros.
+    inv H.
+    destruct a.
+      1-2: inv H.
+      destruct (aeval fuel' a1 s) eqn: H1,
+               (aeval fuel' a2 s) eqn: H2; inv H; eauto.
+      destruct (aeval fuel' a1 s) eqn: H1,
+               (aeval fuel' a2 s) eqn: H2; inv H; eauto.
+      destruct (aeval fuel' a1 s) eqn: H1,
+               (aeval fuel' a2 s) eqn: H2; inv H; eauto.
+      destruct (ceval fuel' c s) eqn: H1; inv H; eauto.
+  destruct fuel as [| fuel']; cbn; intros.
+    inv H.
+    destruct e.
+      1-2: inv H; auto.
+      destruct (aeval fuel' a s) eqn: H1,
+               (aeval fuel' a0 s) eqn: H2; inv H; eauto.
+      destruct (aeval fuel' a s) eqn: H1,
+               (aeval fuel' a0 s) eqn: H2; inv H; eauto.
+      destruct (beval fuel' e s) eqn: H1; inv H; eauto.
+      destruct (beval fuel' e1 s) eqn: H1,
+               (beval fuel' e2 s) eqn: H2; inv H; eauto.
+      destruct (beval fuel' e1 s) eqn: H1,
+               (beval fuel' e2 s) eqn: H2; inv H; eauto.
+  destruct fuel as [| fuel']; cbn; intros.
+    inv H.
+    destruct c.
+      inv H.
+      destruct (aeval fuel' a s1) eqn: H1; inv H; eauto.
+      destruct (ceval fuel' c1 s1) eqn: H1; inv H; eauto.
+      destruct (beval fuel' b s1) eqn: H1.
+        destruct b0; eauto.
+        inv H.
+      destruct (beval fuel' b s1) eqn: H1; inv H.
+        destruct b0; inv H2; eauto.
+        destruct (ceval fuel' c s1) eqn: H; inv H0; eauto.
+Qed.
+
+(*
+Lemma AEval_aeval :
+  forall {fuel : nat} {a : AExp} {s : State} {n : nat},
+    AEval a s n -> aeval fuel a s = n
+
+with BEval_beval :
+  forall {n : nat} {e : BExp} {s : State} {b : bool},
+    BEval e s b -> beval n e s = b
+*)
