make_makefile.sh
@@ -1,2 +1,2 @@
 #!/bin/sh
-coq_makefile -R "." FormalSystems -o makefile *v */*v
+coq_makefile -R "." FormalSystems -o makefile *v */*v */*/*v
